Weidenbach_Book/Pairing_Heap/Heaps_Abs.thy
@@ -91,11 +91,11 @@ begin
       RETURN (v, bw)
       })"
 
-    definition mop_prio_rescale where
-      "mop_prio_rescale = (\<lambda>f (\<A>, b, w). doN {
-      ASSERT (\<forall>x y. le x y \<longleftrightarrow> le (f x) (f y));
-      RETURN (\<A>, b, f o w)
-      })"
+    definition mop_prio_change_all_weights where
+      "mop_prio_change_all_weights \<equiv> (\<lambda>(\<A>, b, w). doN {w \<leftarrow> RES UNIV; RETURN (\<A>, b, w)})"
+
+    definition mop_prio_change_all_weights' where
+      "mop_prio_change_all_weights' _ \<equiv> mop_prio_change_all_weights"
 
 sublocale pairing_heap
   by unfold_locales (rule hm_le hm_trans hm_transt hm_totalt)+
